ROOT
@@ -1914,6 +1914,7 @@ session RRA_Factor_Structural_Bootstrap = HOL +
     Development_Given_Installation
     Development_Rooted_Registrations
     Development_Given_Extensions
+    Development_Given_Carried_Declarations
     Development_Installed_Presentations
     Development_Installed_Presentations_Execution
     Development_First_Problem_Asked
